new autosubst-generated files, now it has the labels syntax

pi.sig
@@ -1,7 +1,7 @@
 -- the types
 chan : Type
 proc : Type
-
+lab: Type
 
 
 -- the constructors for proc
@@ -10,3 +10,13 @@ Par : proc -> proc -> proc
 Rcv : chan -> (bind chan in proc) -> proc
 Send : chan -> chan -> proc -> proc
 Nu : (bind chan in proc) -> proc
+
+
+-- constructors for lab
+Lsend : chan -> chan -> lab 
+Lrcv : chan -> chan -> lab
+LbdSend : chan -> lab
+Ltau : lab
+
+
+
